src/Prototype/Reduction.v
@@ -7,22 +7,19 @@ Section Reduction.
 
   Definition Reduced (from to: list Msg) (msg1 msg2: Msg) :=
     exists hst1 hst2,
-      from = hst1 ++ (msg1 :: msg2 :: hst2) /\
-      to = hst1 ++ (msg2 :: msg1 :: hst2).
+      from = hst1 ++ msg1 :: msg2 :: hst2 /\
+      to = hst1 ++ msg2 :: msg1 :: hst2.
 
-  Lemma reduction_preserved_steps':
+  Lemma reduction_preserves_steps':
     forall msg1 msg2: Msg,
       msg_from msg1 <> msg_from msg2 ->
       forall oss1 oims1 oss2 oims2 hst2 hst1,
         steps oss1 oims1 (hst1 ++ msg1 :: msg2 :: hst2) oss2 oims2 ->
         steps oss1 oims1 (hst1 ++ msg2 :: msg1 :: hst2) oss2 oims2.
   Proof.
-    induction hst1; simpl; intros.
-    - admit.
-    - admit.
   Admitted.
 
-  Theorem reduction_preserved_steps:
+  Theorem reduction_preserves_steps:
     forall oss1 oims1 hst oss2 oims2,
       steps oss1 oims1 hst oss2 oims2 ->
       forall msg1 msg2 hst',
@@ -33,10 +30,45 @@ Section Reduction.
                                            *)
         steps oss1 oims1 hst' oss2 oims2.
   Proof.
-    intros.
     unfold Reduced; intros.
     destruct H0 as [hst1 [hst2 [? ?]]]; subst.
-    apply reduction_preserved_steps'; auto.
+    apply reduction_preserves_steps'; auto.
+  Qed.
+
+  Definition ReducedM (from to msgs: list Msg) (tmsg: Msg) :=
+    exists hst1 hst2,
+      from = hst1 ++ msgs ++ tmsg :: hst2 /\
+      to = hst1 ++ tmsg :: msgs ++ hst2.
+
+  Lemma reductions_preserve_steps':
+    forall (tmsg: Msg) msgs,
+      Forall (fun m => msg_from m <> msg_from tmsg) msgs ->
+      forall oss1 oims1 oss2 oims2 hst2 hst1,
+        steps oss1 oims1 (hst1 ++ msgs ++ tmsg :: hst2) oss2 oims2 ->
+        steps oss1 oims1 (hst1 ++ tmsg :: msgs ++ hst2) oss2 oims2.
+  Proof.
+    induction msgs; simpl; intros; auto.
+
+    replace (hst1 ++ a :: msgs ++ tmsg :: hst2)
+    with ((hst1 ++ a :: nil) ++ msgs ++ tmsg :: hst2) in H0
+      by (repeat rewrite <-app_assoc; reflexivity).
+    inversion_clear H; apply IHmsgs in H0; auto.
+
+    rewrite <-app_assoc in H0; simpl in H0.
+    apply reduction_preserves_steps'; auto.
+  Qed.
+
+  Theorem reductions_preserve_steps:
+    forall oss1 oims1 hst oss2 oims2,
+      steps oss1 oims1 hst oss2 oims2 ->
+      forall msgs tmsg hst',
+        ReducedM hst hst' msgs tmsg ->
+        Forall (fun m => msg_from m <> msg_from tmsg) msgs ->
+        steps oss1 oims1 hst' oss2 oims2.
+  Proof.
+    unfold ReducedM; intros.
+    destruct H0 as [hst1 [hst2 [? ?]]]; subst.
+    apply reductions_preserve_steps'; auto.
   Qed.
 
 End Reduction.
