src/Prototype/Correctness.v
@@ -1,9 +1,6 @@
 Require Import List String Peano_dec.
 Require Import FnMap Language SingleValue.
 
-Theorem impl_serial: SerialObjects impl.
+Theorem impl_linear: Linear impl.
 Proof.
-  unfold SerialObjects, HistoryOf, Serializable; intros.
-  destruct H as [oss [oims ?]].
-
 Admitted.
